safety proof done

ethScript.sml
@@ -60,9 +60,8 @@ Definition in_q1:
 End
 
 Definition in_q2:
-  in_q2 q n = ((q.hd MOD QMAX ≤ n ∧ n < q.tl MOD QMAX) ∨
-                  (q.tl MOD QMAX < q.hd MOD QMAX ∧
-                   (n < q.tl MOD QMAX ∨ q.hd ≤ n MOD QMAX)))
+  in_q2 q n = ((q.hd ≤ n ∧ n < q.tl) ∨
+               (q.tl < q.hd ∧ (n < q.tl ∨ (q.hd ≤ n ∧ n < QMAX))))
 End
 
 (* ALL active entries in the queue must be initialized *)
@@ -103,7 +102,7 @@ Inductive eth:
   ((¬in_q2 q2 n) ⇒ eth (q1, q2) (SOME (Write n p, 0)) (q1, q2 with ps := q2.ps |+ (n, p))) ∧
 
   (* set hd/tl *)
-  (in_q1 q1 n
+  (in_q1 q1 n ∨ n = q1.tl
    ⇒ eth (q1, q2) (SOME (Pop n, 0)) (q1 with hd := n, q2)) ∧
   
   ((¬in_q2 q2 n ∧ (∀i. in_q2 (q2 with tl := n) i ⇒ i ∈ FDOM q2.ps) ∧ n < QMAX)
@@ -113,22 +112,62 @@ Inductive eth:
   (q1.tl - q1.hd < QMAX
    ⇒ eth (q1, q2) NONE ((q1 with ps := q1.ps |+ (q1.tl, n))
                             with tl := q1.tl + 1, q2)) ∧
-  (q2.tl - q2.hd > 0
+  (q2.tl ≠ q2.hd
    ⇒ eth (q1, q2) NONE (q1, q2 with hd := (q2.hd + 1) MOD QMAX))
 End
 
-Theorem qsoundness:
+(* proving that queues are well formed after transitioning *)
+    
+Theorem soundness:
   q1wf q1 ∧ q2wf q2 ∧ eth (q1, q2) e (q1', q2') ⇒ (q1wf q1' ∧ q2wf q2')
 Proof
-  rw[q1wf, q2wf, eth_cases] >> gvs[in_q1, in_q2] >>
-  Cases_on ‘n' < q1.tl’ >> gvs[]
+  rw[q1wf, q2wf, eth_cases] >> gvs[in_q1, in_q2]
+  >- (Cases_on ‘n' < q1.tl’ >> gvs[]) >>
+  Cases_on ‘q2.tl < q2.hd’ >> gvs[] >>
+  Cases_on ‘q2.hd < QMAX - 1’ >> gvs[] >>
+  ‘q2.hd + 1 = QMAX’ by gvs[] >> gvs[]
 QED
+
+Theorem weak_tau_soundness:
+  q1wf q ∧ q2wf r ∧ weak_tau eth (q, r) (q', r') ⇒ q1wf q' ∧ q2wf r'
+Proof
+  fs[weak_tau_def] >>
+  qid_spec_tac ‘q’ >> qid_spec_tac ‘r’ >> 
+  Induct_on ‘RTC’ >>
+  rw[] >> gvs[] >>
+  Cases_on ‘r'³'’ >> 
+  ‘q1wf q'' ∧ q2wf r''’ by metis_tac[soundness] >>
+  gvs[]
+QED
+    
+Theorem weak_trans_soundness:
+  q1wf q1 ∧ q2wf q2 ∧ weak_trans eth (q1, q2) e (q1', q2') ⇒ q1wf q1' ∧ q2wf q2'
+Proof
+  fs[weak_trans_def] >>
+  strip_tac >>
+  Cases_on ‘s'³'’ >> Cases_on ‘s''’ >>
+  ‘q1wf q' ∧ q2wf r'’ by metis_tac[weak_tau_soundness] >>
+  ‘q1wf q ∧ q2wf r’ by metis_tac[soundness] >>
+  metis_tac[weak_tau_soundness]
+QED
+
+Definition length_q1:
+  length_q1 q1 = q1.tl - q1.hd
+End              
+    
+Definition length_q2:
+  length_q2 q2 = if q2.tl ≥ q2.hd then q2.tl - q2.hd else QMAX + q2.tl - q2.hd
+End
+
+    
+(* alternate length_q2: (QMAX + q2.tl - q2.hd) MOD QMAX *)
+
     
 Definition rxdriver:
   rxdriver = Vis Head2 (λx. Vis Tail2
         (λy. Vis Head1 (λz. Vis Tail1
                                 (λw.
-                                   if (w - z = 0 ∨ ((y - x) MOD QMAX) = 0)
+                                   if (w - z = 0 ∨ ((QMAX + y - x + 1) MOD QMAX) = 0)
                                    then Ret ()
                                    else Vis (Read z)
                                    (λa. Vis (Pop (z + 1))
@@ -136,9 +175,588 @@ Definition rxdriver:
                                             (λ_. Vis (Push ((y + 1) MOD QMAX))
                                                      (λ_. Ret ()))))))))
 End
-    
-Theorem rxdriver_safe:
-  safe eth (q1, q2) rxdriver
+
+(* (incomplete) proofs without a notion of length
+
+Theorem none_q2_hd:
+  q2wf (SND s) ∧ q2wf (SND s') ∧ eth s NONE ⇒
+  (SND s).hd = (SND s').hd ∨ ((SND s).hd + 1) MOD QMAX = (SND s').hd ∧ (SND s).hd ≠ (SND s').tl)  
 Proof
+  Cases_on ‘s’ >> Cases_on ‘s'’ >> rw[] >>
+  gvs[Once eth_cases, q2wf]
+QED
+    
+Theorem weak_tau_q2_hd:
+  q1wf q1 ∧ q2wf q2 ∧ q2wf q2' ∧ weak_tau eth (q1,q2) (q1',q2')
+  ⇒ (in_q2 (q2' with hd := q2.hd) q2'.hd ∨
+     q2'.hd = q2'.tl)
+Proof
+  ‘∀q1 q2 q1' q2'. weak_tau eth (q1,q2) (q1',q2') ⇒ q2.tl = q2'.tl’
+  by metis_tac[weak_tau_eq, pairTheory.SND] >>
+  gvs[weak_tau_def] >>
+  qid_spec_tac ‘q2’ >> qid_spec_tac ‘q1’ >> 
+  Induct_on ‘RTC’ >>
+  rw[] >> gvs[in_q2] >>
+  pop_assum mp_tac >> Cases_on ‘q2'³'’ >> gvs[] >> rw[] >>
+  ‘q1wf q ∧ q2wf r’ by metis_tac[soundness] >>
+  ‘q2.hd = r.hd ∨ (q2.hd + 1) MOD QMAX = r.hd ∧ q2.hd ≠ r.tl’
+    by metis_tac[none_q2_hd, pairTheory.SND] >> gvs[] >>
+  Cases_on ‘q2.hd < QMAX - 1’ >> gvs[q2wf]
+  >- (Cases_on ‘q2'.tl < QMAX - 1’ >> gvs[] >>
+      ‘q2.hd = q2'.tl’ by gvs[] >>
+      ‘r.tl = q2'.tl’ by metis_tac[] >> gvs[])
+  >- (Cases_on ‘q2'.tl < q2.hd’ >> gvs[] >>
+      ‘q2'.tl = q2.hd’ by gvs[] >>
+      ‘q2'.tl = r.tl’ by metis_tac[] >> gvs[])
+  >- (Cases_on ‘q2'.tl < q2.hd’ >> gvs[] >>
+      ‘q2'.tl = q2.hd’ by gvs[] >>
+      ‘q2'.tl = r.tl’ by metis_tac[] >> gvs[])
+  >- (‘q2.hd = QMAX - 1’ by gvs[q2wf] >>
+      ‘r.hd = 0’ by gvs[q2wf] >> gvs[])
+QED
+
+Theorem weak_trans_head2:
+  q1wf q1' ∧ q2wf q2' ∧ q2wf r ∧ weak_trans eth (q1', q2') (Head2, b) (q, r)
+  ⇒ (in_q2 (r with hd := b) r.hd ∨ r.hd = r.tl)
+Proof
+  rw[Once weak_trans_def] >>
+  Cases_on ‘s''’ >> Cases_on ‘s'³'’ >>
+  irule weak_tau_q2_hd >>
+  ‘q1wf (FST (q1', q2')) ∧ q2wf (SND (q1', q2')) ∧ weak_tau eth (q1', q2') (q', r')
+   ⇒ (q1wf (FST (q', r')) ∧ q2wf (SND (q', r')))’
+    by metis_tac[weak_tau_soundness] >> gvs[] >>
+  ‘q1wf q'' ∧ q2wf r''’ by metis_tac[soundness] >> metis_tac[]
+QED
+
+Theorem weak_tau_in_q2_hd:
+  in_q2 (q2 with hd := x) q2.hd ∧ weak_tau eth (q1, q2) (q, r) ∧
+  q1wf q1' ∧ q2wf q2' ∧ q1wf q ∧ q2wf r ⇒
+  in_q2 (r with hd := x) r.hd ∨ r.hd = r.tl
+Proof
+  fs[weak_tau_def] >>
+  qid_spec_tac ‘q2’ >> qid_spec_tac ‘q1’ >> 
+  Induct_on ‘RTC’ >> rw[] >> gvs[in_q2]
+  >- ()
+QED
+    
+Theorem weak_trans_tail2:
+  in_q2 (q2' with hd := x) q2'.hd ∧ weak_trans eth (q1', q2') (Tail2, b) (q, r) ∧
+  q1wf q1 ∧ q2wf q2 ∧ q1wf q1' ∧ q2wf q2'∧ q1wf q ∧ q2wf r ⇒
+  in_q2 (r with hd := x) r.hd ∨ r.hd = r.tl
+Proof
+  rw[weak_trans_def] >>
+  Cases_on ‘s''’ >> Cases_on ‘s'³'’ >>
+  ‘q'' = q' ∧ r'' = r'’ by gvs[eth_cases] >> gvs[] >>
+QED *)
+
+(* proofs about length notions *)
+
+Theorem weak_tau_eq:
+  weak_tau eth (q, r) (q', r') ⇒ r.tl = r'.tl ∧ q.hd = q'.hd
+Proof
+  fs[weak_tau_def] >>
+  qid_spec_tac ‘q’ >> qid_spec_tac ‘r’ >>
+  Induct_on ‘RTC’ >> rw[] >>
+  Cases_on ‘r'³'’ >>
+  qpat_x_assum ‘_꙳ _ _’ kall_tac >>
+  gvs[eth_cases]
+QED
+   
+(* theorems about q2 length and with hd *)
+
+Theorem none_length_with_hd:
+  eth (q, r) NONE (q', r') ⇒ length_q2 (r' with hd := r.hd) = length_q2 r
+Proof
+  rw[] >>
+  ‘r.tl = r'.tl’ by fs[eth_cases] >>
+  gvs[eth_cases, length_q2]
+QED
+    
+Theorem weak_tau_length_with_hd:
+  weak_tau eth (q, r) (q', r') ⇒ length_q2 (r' with hd := r.hd) = length_q2 r
+Proof
+  fs[weak_tau_def] >>
+  qid_spec_tac ‘q'’ >> qid_spec_tac ‘r'’ >>
+  Induct_on ‘RTC’ using RTC_INDUCT_RIGHT1 >>
+  rw[] >- gvs[length_q2] >>
+  Cases_on ‘s’ >>
+  ‘r'.tl = r''.tl’ by fs[eth_cases] >>
+  gvs[length_q2]          
+QED
+
+(* theorems about how q2 length changes with transitions *)
+    
+Theorem none_length_q2:
+  q2wf q2 ∧ q2wf q2' ∧ eth (q1, q2) NONE (q1', q2') ⇒
+  length_q2 q2 = length_q2 q2' ∨ length_q2 q2 = length_q2 q2' + 1
+Proof
+  rw[q2wf, length_q2] >> gvs[eth_cases] >>
+  Cases_on ‘q2.hd < QMAX - 1’ >> gvs[] >>
+  ‘q2.hd + 1 = QMAX’ by rw[] >> gvs[]
+QED
+
+Theorem weak_tau_length_q2:
+  weak_tau eth (q, r) (q', r') ∧
+  q1wf q' ∧ q2wf r' ∧ q1wf q ∧ q2wf r
+  ⇒ length_q2 r ≥ length_q2 r'
+Proof
+  fs[weak_tau_def] >>
+  qid_spec_tac ‘q’ >> qid_spec_tac ‘r’ >>
+  Induct_on ‘RTC’ >> rw[] >- rw[] >>
+  Cases_on ‘r'³'’ >>
+  ‘q1wf q'' ∧ q2wf r''’ by metis_tac[soundness] >> gvs[] >>
+  ‘length_q2 r = length_q2 r'' ∨ length_q2 r = length_q2 r'' + 1’
+    by metis_tac[none_length_q2] >> gvs[]
+QED
+    
+Theorem weak_trans_length_head2:
+  weak_trans eth (q1, q2) (Head2, b) (q, r) ∧
+  q1wf q1 ∧ q2wf q2 ∧ q1wf q ∧ q2wf r
+  ⇒ length_q2 (r with hd := b) ≥ length_q2 r
+Proof
+  rw[weak_trans_def] >> Cases_on ‘s''’ >>
+  ‘s'³' = (q', r') ∧ b = r'.hd’ by gvs[eth_cases] >>
+  ‘q1wf q' ∧ q2wf r'’ by metis_tac[weak_tau_soundness] >>
+  metis_tac[weak_tau_length_q2, weak_tau_length_with_hd]
+QED
+
+Theorem weak_trans_length_rest:
+  e ∈ {Tail2; Head1; Tail1; Read a} ∧
+  length_q2 (q2' with hd := x) ≥ length_q2 q2' ∧
+  weak_trans eth (q1', q2') (e, b) (q, r) ∧
+  q1wf q1' ∧ q2wf q2' ∧ q1wf q ∧ q2wf r
+  ⇒ length_q2 (r with hd := x) ≥ length_q2 r
+Proof
+  rw[weak_trans_def] >> Cases_on ‘s''’ >>
+  ‘s'³' = (q', r')’ by gvs[eth_cases] >>
+  ‘q1wf q' ∧ q2wf r'’ by metis_tac[weak_tau_soundness] >>
+  ‘r'.tl = r.tl ∧ q2'.tl = r'.tl’ by metis_tac[weak_tau_eq] >>
+  ‘length_q2 (q2' with hd := x) = length_q2 (r with hd := x)’ by gvs[length_q2] >>
+  ‘length_q2 q2' ≥ length_q2 r' ∧ length_q2 r' ≥ length_q2 r’
+    by metis_tac[weak_tau_length_q2] >>
+  rw[]
+QED
+
+(* theorems about constant values from function calls *)
+
+Theorem tail_2:
+  weak_trans eth (q, r) (Tail2, b) (q', r') ⇒ r'.tl = b
+Proof
+  rw[weak_trans_def] >>
+  Cases_on ‘s'³'’ >>
+  ‘r'.tl = r''.tl’ by metis_tac[weak_tau_eq] >>
+  gvs[eth_cases]
+QED
+
+Theorem head_1:
+  weak_trans eth (q, r) (Head1, b) (q', r') ⇒ b = q'.hd
+Proof
+  rw[weak_trans_def] >>
+  Cases_on ‘s'³'’ >>
+  ‘s'' = (q'', r'')’ by gvs[eth_cases] >> rw[] >>
+  ‘b = q''.hd’ by gvs[eth_cases] >>
+  ‘q''.hd = q'.hd’ by metis_tac[weak_tau_eq] >> gvs[]
+QED
+    
+Theorem weak_trans_eq:
+  e ∈ {Head1; Head2; Tail1; Tail2; Read a} ∧
+  weak_trans eth (q, r) (e, b) (q', r')
+  ⇒ q.hd = q'.hd ∧ r.tl = r'.tl                                                    
+Proof
+  rw[weak_trans_def] >>
+  Cases_on ‘s'³'’ >>
+  ‘s'' = (q'', r'')’ by gvs[eth_cases] >> rw[] >>
+  ‘r'.tl = r''.tl ∧ r.tl = r''.tl ∧ q'.hd = q''.hd ∧ q.hd = q''.hd’
+  by metis_tac[weak_tau_eq] >> gvs[]
+QED
+
+(* theorems about q1 *)
+
+Theorem weak_tau_q1_tl:
+  weak_tau eth (q, r) (q', r') ⇒ q.tl ≤ q'.tl
+Proof
+  fs[weak_tau_def] >>
+  qid_spec_tac ‘q’ >> qid_spec_tac ‘r’ >>
+  Induct_on ‘RTC’ >> rw[] >- rw[] >>
+  Cases_on ‘r'³'’ >>
+  qpat_x_assum ‘_꙳ _ _’ kall_tac >>
+  gvs[eth_cases]
+QED               
+  
+Theorem tail_1:
+  weak_trans eth (q, r) (Tail1, b) (q', r') ⇒ b ≤ q'.tl
+Proof
+  rw[weak_trans_def] >>
+  Cases_on ‘s'³'’ >>
+  ‘b = q''.tl’ by gvs[eth_cases] >>
+  ‘q''.tl ≤ q'.tl’ by metis_tac[weak_tau_q1_tl] >>          
+  simp[]
+QED
+    
+Theorem weak_trans_q1_tl:
+  e ∈ {Read a} ∧ weak_trans eth (q, r) (e, b) (q', r') ⇒ q.tl ≤ q'.tl
+Proof
+  rw[weak_trans_def] >>
+  Cases_on ‘s'³'’ >>
+  ‘s'' = (q'', r'')’ by gvs[eth_cases] >> rw[] >>
+  ‘q.tl ≤ q''.tl ∧ q''.tl ≤ q'.tl’ by metis_tac[weak_tau_q1_tl] >>
+  simp[]
+QED
+
+(* for popping *)
+
+Theorem pop_q2_tl:
+  weak_trans eth (q, r) (Pop (q.hd + 1), b) (q', r') ⇒ r.tl = r'.tl
+Proof
+  rw[weak_trans_def] >> Cases_on ‘s'³'’ >> Cases_on ‘s''’ >>
+  ‘r'³' = r''’ by gvs[eth_cases] >> rw[] >>
+  ‘r.tl = r''.tl ∧ r''.tl = r'.tl’ by metis_tac[weak_tau_eq] >> simp[]
+QED
+
+Theorem pop_q1_tl:
+  weak_trans eth (q, r) (Pop (q.hd + 1), b) (q', r') ⇒ q.tl ≤ q'.tl
+Proof
+  rw[weak_trans_def] >> Cases_on ‘s'³'’ >> Cases_on ‘s''’ >>
+  ‘q.tl ≤ q'³'.tl ∧ q''.tl ≤ q'.tl’ by metis_tac[weak_tau_q1_tl] >>
+  ‘q'³'.tl ≤ q''.tl’ by gvs[eth_cases] >> simp[]
+QED
+    
+Theorem pop_q2_length:
+  length_q2 (r with hd := x) ≥ length_q2 r ∧
+  weak_trans eth (q, r) (Pop (q.hd + 1), b) (q', r') ∧
+  q1wf q ∧ q2wf r ∧ q1wf q' ∧ q2wf r'
+  ⇒ length_q2 (r' with hd := x) ≥ length_q2 r'
+Proof
+  rw[weak_trans_def] >> Cases_on ‘s''’ >> Cases_on ‘s'³'’ >>
+  ‘r'³' = r''’ by gvs[eth_cases] >> rw[] >>
+  ‘q1wf q'' ∧ q2wf r''’ by metis_tac[weak_tau_soundness] >>
+  ‘q1wf q'³'’ by metis_tac[soundness] >>
+  ‘r''.tl = r.tl ∧ r''.tl = r'.tl’ by metis_tac[weak_tau_eq] >>
+  ‘length_q2 (r' with hd := x) = length_q2 (r with hd := x)’ by gvs[length_q2] >>          
+  ‘length_q2 r ≥ length_q2 r'' ∧ length_q2 r'' ≥ length_q2 r'’
+    by metis_tac[weak_tau_length_q2] >> rw[]
+QED
+
+(* for pushing *)
+
+Theorem push_tl:
+  weak_trans eth (q, r) (Write x y, b) (q', r') ⇒ r.tl = r'.tl ∧ q.tl ≤ q'.tl
+Proof
+  rw[weak_trans_def] >> Cases_on ‘s''’ >> Cases_on ‘s'³'’
+  >- (‘r''.tl = r'³'.tl’ by gvs[eth_cases] >>
+      ‘r''.tl = r.tl ∧ r''.tl = r'.tl’ by metis_tac[weak_tau_eq] >> simp[])
+  >- (‘q'' = q'³'’ by gvs[eth_cases] >>
+      ‘q.tl ≤ q''.tl ∧ q''.tl ≤ q'.tl’ by metis_tac[weak_tau_q1_tl] >> simp[])     
+QED
+    
+Theorem push_q2_length:
+  length_q2 (r with hd := x) ≥ length_q2 r ∧
+  weak_trans eth (q, r) (Write n m, b) (q', r') ∧
+  q1wf q ∧ q2wf r ∧ q1wf q' ∧ q2wf r'
+  ⇒ length_q2 (r' with hd := x) ≥ length_q2 r'
+Proof
+  rw[weak_trans_def] >> Cases_on ‘s''’ >> Cases_on ‘s'³'’ >>
+  ‘r'³'.tl = r''.tl ∧ r'³'.hd = r''.hd’ by gvs[eth_cases] >> rw[] >>
+  ‘q1wf q'' ∧ q2wf r''’ by metis_tac[weak_tau_soundness] >>
+  ‘q1wf q'³' ∧ q2wf r'³'’ by metis_tac[soundness] >>
+  ‘r''.tl = r.tl ∧ r''.tl = r'.tl’ by metis_tac[weak_tau_eq] >>
+  ‘length_q2 (r' with hd := x) = length_q2 (r with hd := x)’ by gvs[length_q2] >>          
+  ‘length_q2 r ≥ length_q2 r'' ∧ length_q2 r'³' ≥ length_q2 r'’
+    by metis_tac[weak_tau_length_q2] >>
+  ‘length_q2 r'' = length_q2 r'³'’ by metis_tac[length_q2] >> simp[]
+QED
+
+(* random domain stuff for the final cases *)
+    
+Theorem weak_tau_dom:
+  weak_tau eth (q', r') (q, r) ∧ a ∈ FDOM r'.ps ⇒ a ∈ FDOM r.ps
+Proof
+  fs[weak_tau_def] >>
+  qid_spec_tac ‘r'’ >> qid_spec_tac ‘q'’ >>
+  Induct_on ‘RTC’ >> rw[] >- rw[] >>
+  Cases_on ‘r'³'’ >> rw[] >>
+  ‘a ∈ FDOM r''.ps’ by gvs[eth_cases] >> simp[]
+QED
+    
+Theorem write_dom:
+  weak_trans eth (q1', q2') (Write r.tl a, b) (q, r)
+  ⇒ r.tl ∈ FDOM r.ps
+Proof
+  rw[weak_trans_def] >> Cases_on ‘s'³'’ >> Cases_on ‘s''’ >>
+  ‘r.tl ∈ FDOM r'.ps’ by gvs[eth_cases] >>
+  metis_tac[weak_tau_dom]
+QED
+
+(* oh god its more length theorems *)
+
+Theorem max_length_q2:
+  q2wf q ⇒ length_q2 q < QMAX
+Proof
+  gvs[length_q2, q2wf]
+QED
+
+Theorem head2_max_length:
+  weak_trans eth (q, r) (Head2, b) (q', r') ∧ q1wf q ∧ q2wf r
+  ⇒ QMAX > length_q2 (r' with hd := b)
+Proof
+  rw[weak_trans_def] >>
+  Cases_on ‘s'³'’ >>
+  ‘s'' = (q'', r'')’ by gvs[eth_cases] >>
+  ‘b = r''.hd’ by gvs[eth_cases] >>
+  ‘r''.tl = r'.tl’ by metis_tac[weak_tau_eq] >>
+  ‘length_q2 (r' with hd := r''.hd) = length_q2 r''’ by gvs[length_q2] >>
+  ‘q2wf r''’ by metis_tac[weak_tau_soundness] >> gvs[] >>
+        drule max_length_q2 >> simp[]
+QED
+    
+Theorem remaining_max_length:
+  e ∈ {Tail2; Head1; Tail1; Read a; Write n m; Pop c} ∧
+  QMAX > length_q2 (r with hd := x) ∧
+  weak_trans eth (q, r) (e, b) (q', r')
+  ⇒ QMAX > length_q2 (r' with hd := x)
+Proof
+  rw[weak_trans_def] >>
+  Cases_on ‘s'³'’ >> Cases_on ‘s''’ >>
+  ‘r''.tl = r'³'.tl’ by gvs[eth_cases] >>
+  ‘r.tl = r'³'.tl ∧ r''.tl =  r'.tl’ by metis_tac[weak_tau_eq] >>
+  gvs[length_q2]
+QED
+     
+Theorem weak_tau_not_in_q2:
+  q1wf q ∧ q2wf r ∧
+  QMAX > length_q2 (r with hd := x) ∧
+  weak_tau eth (q, r) (q', r') ∧
+  length_q2 (r with hd := x) ≥ length_q2 r ∧
+  (QMAX + r.tl - x + 1) MOD QMAX ≠ 0
+  ⇒ ¬in_q2 r' ((r.tl + 1) MOD QMAX)
+Proof
+  rw[] >>
+  ‘r.tl = r'.tl’ by metis_tac[weak_tau_eq] >>
+  ‘q1wf q' ∧ q2wf r'’ by metis_tac[weak_tau_soundness] >>
+  ‘length_q2 r ≥ length_q2 r'’ by metis_tac[weak_tau_length_q2] >>
+  Cases_on ‘r.tl + 1 < QMAX’ >> gvs[q2wf, in_q2]
+  >- (Cases_on ‘¬(r'.tl < r'.hd) ∨ ¬(r'.hd ≤ r'.tl + 1)’ >> gvs[] >>
+      ‘r'.hd = r'.tl + 1’ by gvs[] >>
+      subgoal ‘length_q2 r' = QMAX - 1’
+      >- gvs[length_q2] >>
+      ‘length_q2 (r with hd := x) = QMAX - 1’ by gvs[] >>
+      Cases_on ‘r'.tl ≥ x’ >> gvs[length_q2])
+  >- (‘r'.tl + 1 = QMAX’ by gvs[] >> 
+      Cases_on ‘¬(r'.hd ≤ (r'.tl + 1) MOD QMAX) ∨ ¬((r'.tl + 1) MOD QMAX < r'.tl)’ >>
+      gvs[] >>
+      ‘length_q2 r' = QMAX - 1’ by gvs[length_q2] >>
+      ‘length_q2 (r with hd := x) = QMAX - 1’ by gvs[] >>
+      Cases_on ‘r'.tl ≥ x’ >> gvs[length_q2] >>
+      ‘x = 0’ by gvs[] >> gvs[])
+QED
+
+Theorem in_q2_plus_1:
+  length_q2 r < QMAX - 1 ∧ q2wf r ∧
+  in_q2 (r with tl := (r.tl + 1) MOD QMAX) i
+  ⇒ in_q2 r i ∨ i = r.tl
+Proof
+  rw[] >>
+  gvs[in_q2, q2wf, length_q2] >>
+  Cases_on ‘r.tl + 1 = QMAX’ >> gvs[]
+QED
+    
+Theorem weak_tau_in_q2_dom:
+  length_q2 r < QMAX - 1 ∧
+  r.tl ∈ FDOM r.ps ∧ q2wf r ⇒
+  (∀i. in_q2 (r with tl := (r.tl + 1) MOD QMAX) i ⇒ i ∈ FDOM r.ps)
+Proof
+  rw[] >>
+  ‘in_q2 r i ∨ i = r.tl’ by metis_tac[in_q2_plus_1] >>
+  gvs[q2wf]
+QED
+  
+Theorem weak_tau_in_in_q2:
+  length_q2 r < QMAX - 1 ∧
+  in_q2 (r' with tl := (r.tl + 1) MOD QMAX) i ∧
+  weak_tau eth (q, r) (q', r') ∧ q2wf r ∧ q2wf r' ∧ q1wf q ∧ q1wf q' 
+  ⇒ in_q2 (r with tl := (r.tl + 1) MOD QMAX) i
+Proof
+  rw[] >>
+  ‘r.tl = r'.tl’ by metis_tac[weak_tau_eq] >> gvs[] >>
+  ‘length_q2 r ≥ length_q2 r'’ by metis_tac[weak_tau_length_q2] >>
+  rw[in_q2, q2wf] >> gvs[length_q2] >>
+  Cases_on ‘r'.tl + 1 = QMAX’ >>
+  Cases_on ‘r'.tl ≥ r.hd’ >> gvs[in_q2, q2wf]
+QED  
+
+Theorem q2_inherit:
+  length_q2 r < QMAX - 1 ∧
+  weak_tau eth (q, r) (q', r') ∧
+  q2wf r ∧ q2wf r' ∧ q1wf q ∧ q1wf q' ∧                                      
+  (∀i. in_q2 (r with tl := (r.tl + 1) MOD QMAX) i ⇒ i ∈ FDOM r.ps)
+  ⇒ (∀i. in_q2 (r' with tl := (r.tl + 1) MOD QMAX) i ⇒ i ∈ FDOM r'.ps)
+Proof
+  rw[] >> metis_tac[weak_tau_in_in_q2, weak_tau_dom]
+QED   
+
+Theorem not_max_length:
+  QMAX > length_q2 (r with hd := x) ∧
+  length_q2 (r with hd := x) ≥ length_q2 r ∧
+  (QMAX + r.tl - x + 1) MOD QMAX ≠ 0 ∧ q2wf r
+  ⇒ length_q2 r < QMAX - 1
+Proof
+  rw[] >>
+  Cases_on ‘length_q2 r < QMAX - 1’ >> simp[] >>
+  ‘length_q2 (r with hd := x) = QMAX - 1’ by gvs[] >>
+  gvs[q2wf] 
+  >- (Cases_on ‘r.tl ≥ x’
+      >- (‘QMAX + r.tl - x + 1 = 2 * QMAX’ by gvs[length_q2] >> gvs[])
+      >- fs[length_q2])
+  >- (Cases_on ‘r.tl ≥ x’
+      >- (‘QMAX + r.tl - x + 1 = 2 * QMAX’ by gvs[length_q2] >> gvs[])
+      >- fs[length_q2])
+QED
+
+
+Theorem rxdriver_safe:
+  q1wf q1 ∧ q2wf q2 ⇒ safe eth (q1, q2) rxdriver
+Proof
+  rw[] >>
   irule safe_coind >>
-  qexists ‘’
+  qexists_tac ‘λm s t. ∃q1' q2'. q1wf q1' ∧ q2wf q2' ∧ m = eth ∧ s = (q1', q2') ∧
+                             (t = rxdriver ∨ t = Ret () ∨
+                              (∃x. length_q2 (q2' with hd := x) ≥ length_q2 q2' ∧
+                                   QMAX > length_q2 (q2' with hd := x) ∧
+                              t = Vis Tail2 (λy. Vis Head1 (λz. Vis Tail1 (λw.
+                                  if (w - z = 0 ∨ ((QMAX + y - x + 1) MOD QMAX) = 0)
+                                  then Ret ()
+                                  else Vis (Read z) (λa. Vis (Pop (z + 1))
+                                  (λ_. Vis (Write y a) (λ_. Vis (Push ((y + 1) MOD QMAX))
+                                                                (λ_. Ret ())))))))) ∨
+                              (∃x. length_q2 (q2' with hd := x) ≥ length_q2 q2' ∧
+                                   QMAX > length_q2 (q2' with hd := x) ∧
+                              t = Vis Head1 (λz. Vis Tail1 (λw.
+                                  if (w - z = 0 ∨ ((QMAX + q2'.tl - x + 1) MOD QMAX) = 0)
+                                  then Ret ()
+                                  else Vis (Read z) (λa. Vis (Pop (z + 1))
+                                  (λ_. Vis (Write q2'.tl a) (λ_. Vis (Push ((q2'.tl + 1) MOD QMAX))
+                                                                     (λ_. Ret ()))))))) ∨
+                              (∃x. length_q2 (q2' with hd := x) ≥ length_q2 q2' ∧
+                                   QMAX > length_q2 (q2' with hd := x) ∧
+                              t = Vis Tail1 (λw.
+                                  if (w - q1'.hd = 0 ∨ ((QMAX + q2'.tl - x + 1) MOD QMAX) = 0)
+                                  then Ret ()
+                                  else Vis (Read q1'.hd) (λa. Vis (Pop (q1'.hd + 1))
+                                  (λ_. Vis (Write q2'.tl a) (λ_. Vis (Push ((q2'.tl + 1) MOD QMAX))
+                                                                     (λ_. Ret ())))))) ∨
+                              (∃x w. length_q2 (q2' with hd := x) ≥ length_q2 q2' ∧
+                                     QMAX > length_q2 (q2' with hd := x) ∧
+                                     (w ≤ q1'.tl) ∧
+                              t = if (w - q1'.hd = 0 ∨ ((QMAX + q2'.tl - x + 1) MOD QMAX) = 0)
+                                  then Ret ()
+                                  else Vis (Read q1'.hd) (λa. Vis (Pop (q1'.hd + 1))
+                                  (λ_. Vis (Write q2'.tl a) (λ_. Vis (Push ((q2'.tl + 1) MOD QMAX))
+                                                                     (λ_. Ret ()))))) ∨
+                              (∃x w. length_q2 (q2' with hd := x) ≥ length_q2 q2' ∧
+                                     QMAX > length_q2 (q2' with hd := x) ∧
+                                     (w ≤ q1'.tl) ∧
+                                   ¬(w - q1'.hd = 0 ∨ ((QMAX + q2'.tl - x + 1) MOD QMAX) = 0) ∧
+                              t = Vis (Read q1'.hd) (λa. Vis (Pop (q1'.hd + 1))
+                             (λ_. Vis (Write q2'.tl a) (λ_. Vis (Push ((q2'.tl + 1) MOD QMAX))
+                                                                (λ_. Ret ()))))) ∨
+                              (∃x w a. length_q2 (q2' with hd := x) ≥ length_q2 q2' ∧
+                                       QMAX > length_q2 (q2' with hd := x) ∧
+                                       (w ≤ q1'.tl) ∧
+                                       ¬(w - q1'.hd = 0 ∨ ((QMAX + q2'.tl - x + 1) MOD QMAX) = 0) ∧
+                              t = Vis (Pop (q1'.hd + 1))
+                             (λ_. Vis (Write q2'.tl a) (λ_. Vis (Push ((q2'.tl + 1) MOD QMAX))
+                                                                (λ_. Ret ())))) ∨
+                              (∃x w a. length_q2 (q2' with hd := x) ≥ length_q2 q2' ∧
+                                       QMAX > length_q2 (q2' with hd := x) ∧
+                                       (w ≤ q1'.tl) ∧
+                                       ¬(((QMAX + q2'.tl - x + 1) MOD QMAX) = 0) ∧
+                              t = Vis (Write q2'.tl a) (λ_. Vis (Push ((q2'.tl + 1) MOD QMAX))
+                                                                (λ_. Ret ()))) ∨
+                              (∃x w a. length_q2 (q2' with hd := x) ≥ length_q2 q2' ∧
+                                       QMAX > length_q2 (q2' with hd := x) ∧
+                                       (w ≤ q1'.tl) ∧
+                                       ¬(((QMAX + q2'.tl - x + 1) MOD QMAX) = 0) ∧
+                                       q2'.tl ∈ FDOM q2'.ps ∧
+                              t = Vis (Push ((q2'.tl + 1) MOD QMAX))
+                                      (λ_. Ret ())))’ >>
+  rw[]
+  >- (rpt $ disj2_tac >> rw[Once rxdriver] >>
+      Cases_on ‘s'’ >> gvs[eth_cases] >>
+      ‘q1wf q ∧ q2wf r’ by metis_tac[weak_trans_soundness] >> rw[] >>
+      disj2_tac >> disj1_tac >> qexists ‘b’ >> gvs[] >>
+      metis_tac[weak_trans_length_head2, head2_max_length])
+  >- (rw[] >> Cases_on ‘s'’ >> gvs[eth_cases] >>
+      ‘q1wf q ∧ q2wf r’ by metis_tac[weak_trans_soundness] >> rw[] >>
+      disj2_tac >> disj1_tac >> qexists ‘x’ >> gvs[] >> rw[]
+      >- (irule weak_trans_length_rest >> fs[] >> metis_tac[]) >>
+      ‘b = r.tl’ by metis_tac[tail_2] >> gvs[] >>
+      irule remaining_max_length >> fs[] >> metis_tac[])
+  >- (rw[] >> Cases_on ‘s'’ >> gvs[eth_cases] >>
+      ‘q1wf q ∧ q2wf r’ by metis_tac[weak_trans_soundness] >> rw[] >>
+      disj2_tac >> disj1_tac >> qexists ‘x’ >> gvs[] >> rw[]
+      >- (irule weak_trans_length_rest >> fs[] >>  metis_tac[]) >>
+      ‘b = q.hd’ by metis_tac[head_1] >>
+      subgoal ‘q1'.hd = q.hd ∧ q2'.tl = r.tl’
+      >- (irule weak_trans_eq >> fs[] >> metis_tac[]) >> gvs[]
+      >- (irule remaining_max_length >> fs[] >> metis_tac[]) >>
+      irule weak_trans_eq >> fs[] >> metis_tac[])
+  >- (rw[] >> Cases_on ‘s'’ >> gvs[eth_cases] >>
+      ‘q1wf q ∧ q2wf r’ by metis_tac[weak_trans_soundness] >> rw[] >>
+      rpt $ disj2_tac >> qexistsl [‘x’, ‘b’] >> rw[]
+      >- (irule weak_trans_length_rest >> fs[] >> metis_tac[])
+      >- (irule remaining_max_length >> fs[] >> metis_tac[]) >>
+      subgoal ‘q1'.hd = q.hd ∧ q2'.tl = r.tl’
+      >- (irule weak_trans_eq >> fs[] >> metis_tac[]) >> gvs[]                                                 
+      >- metis_tac[tail_1] >>
+      irule weak_trans_eq >> fs[] >> metis_tac[])
+  >- (Cases_on ‘w ≤ q1'.hd ∨ (QMAX + q2'.tl − x + 1) MOD QMAX = 0’ >> gvs[] >>
+      rw[] >> Cases_on ‘s'’ >> gvs[eth_cases]
+      >- (‘q.hd = q1'.hd’ by metis_tac[weak_tau_eq] >>
+          ‘q1'.tl ≤ q.tl’ by metis_tac[weak_tau_q1_tl] >> gvs[in_q1]) >>
+      ‘q1wf q ∧ q2wf r’ by metis_tac[weak_trans_soundness] >> rw[] >>
+      rpt $ disj2_tac >> qexistsl [‘x’, ‘w’, ‘b’] >>
+      subgoal ‘QMAX > length_q2 (r with hd := x)’
+      >- (irule remaining_max_length >> fs[] >> metis_tac[]) >> simp[] >>
+      subgoal ‘q1'.hd = q.hd ∧ q2'.tl = r.tl’
+      >- (irule weak_trans_eq >> fs[] >> metis_tac[]) >> gvs[] >> rw[]
+      >- (irule weak_trans_length_rest >> fs[] >> metis_tac[]) >>
+      subgoal ‘q1'.tl ≤ q.tl’
+      >- (irule weak_trans_q1_tl >> fs[] >> metis_tac[]) >> simp[])
+  >- (rw[] >> Cases_on ‘s'’ >> gvs[eth_cases]
+      >- (‘q.hd = q1'.hd’ by metis_tac[weak_tau_eq] >>  
+          ‘q1'.tl ≤ q.tl’ by metis_tac[weak_tau_q1_tl] >> gvs[in_q1]) >>
+      ‘q1wf q ∧ q2wf r’ by metis_tac[weak_trans_soundness] >> rw[] >>
+      rpt $ disj2_tac >> qexistsl [‘x’, ‘w’, ‘b’] >>
+      subgoal ‘QMAX > length_q2 (r with hd := x)’
+      >- (irule remaining_max_length >> fs[] >> metis_tac[]) >> simp[] >>
+      subgoal ‘q1'.hd = q.hd ∧ q2'.tl = r.tl’
+      >- (irule weak_trans_eq >> fs[] >> metis_tac[]) >> gvs[] >> rw[]
+      >- (irule weak_trans_length_rest >> fs[] >> metis_tac[]) >>
+      subgoal ‘q1'.tl ≤ q.tl’
+      >- (irule weak_trans_q1_tl >> fs[] >> metis_tac[]) >> simp[])
+  >- (rw[] >> Cases_on ‘s'’ >> gvs[eth_cases]
+      >- (Cases_on ‘q1'.hd + 1 = q.tl’ >> gvs[in_q1] >>
+          ‘q1'.hd = q.hd’ by metis_tac[weak_tau_eq] >>
+          ‘q1'.tl ≤ q.tl’ by metis_tac[weak_tau_q1_tl] >> gvs[]) >>
+      ‘q1wf q ∧ q2wf r’ by metis_tac[weak_trans_soundness] >> rw[] >>
+      rpt $ disj2_tac >> qexistsl [‘x’, ‘w’] >>
+      subgoal ‘QMAX > length_q2 (r with hd := x)’
+      >- (irule remaining_max_length >> fs[] >> metis_tac[]) >> simp[] >>
+      ‘q2'.tl = r.tl’ by metis_tac[pop_q2_tl] >> fs[] >>
+      ‘q1'.tl ≤ q.tl’ by metis_tac[pop_q1_tl] >> simp[] >>
+      metis_tac[pop_q2_length])
+  >- (rw[] >> Cases_on ‘s'’ >> gvs[eth_cases]
+      >- (‘r.tl = q2'.tl’ by metis_tac[weak_tau_eq] >> gvs[in_q2]) >>
+      ‘q1wf q ∧ q2wf r’ by metis_tac[weak_trans_soundness] >> rw[] >>
+      rpt $ disj2_tac >> qexistsl [‘x’, ‘w’] >>
+      subgoal ‘QMAX > length_q2 (r with hd := x)’
+      >- (irule remaining_max_length >> fs[] >> metis_tac[]) >> simp[] >>
+      ‘q2'.tl = r.tl ∧ q1'.tl ≤ q.tl’ by metis_tac[push_tl] >> fs[] >>
+      metis_tac[push_q2_length, write_dom])
+  >- (rw[] >> Cases_on ‘s'’ >> gvs[eth_cases]
+      >- (‘¬in_q2 r ((q2'.tl + 1) MOD QMAX)’ by metis_tac[weak_tau_not_in_q2] >> simp[] >>
+          ‘length_q2 q2' < QMAX - 1’ by metis_tac[not_max_length] >>
+          ‘q1wf q ∧ q2wf r’ by metis_tac[weak_tau_soundness] >> 
+          metis_tac[weak_tau_in_q2_dom, q2_inherit]) >>
+      ‘q1wf q ∧ q2wf r’ by metis_tac[weak_trans_soundness] >> rw[])       
+QED
